mlanguage + associated WP: switch to semantics with dual nondeterminism

theories/mlanguage/mlanguage.v
@@ -1,6 +1,7 @@
 From stdpp Require Import relations strings gmap.
 From iris.algebra Require Import ofe.
 From iris.prelude Require Import options.
+From melocoton Require Export multirelations.
 
 Section mlanguage_mixin.
   Context {expr val func ectx public_state private_state state : Type}.
@@ -23,7 +24,7 @@ Section mlanguage_mixin.
   Local Notation mixin_prog := (gmap string func).
 
   Context (apply_func : func → list val → option expr).
-  Context (head_step : mixin_prog → expr → state → expr → state → Prop).
+  Context (head_step : mixin_prog → umrel (expr * state)).
 
   Record MlanguageMixin := {
     (** Expression classification *)
@@ -32,12 +33,12 @@ Section mlanguage_mixin.
 
     (** Reduction behavior of the special classes of expressions *)
     (** mixin_val_head_step is not an iff because the backward direction is trivial *)
-    mixin_val_head_step p v σ1 e2 σ2 :
-      head_step p (of_class (ExprVal v)) σ1 e2 σ2 → False;
-    mixin_call_head_step p f vs σ1 e2 σ2 :
-      head_step p (of_class (ExprCall f vs)) σ1 e2 σ2 ↔
-      ∃ (fn : func),
-        p !! f = Some fn ∧ Some e2 = apply_func fn vs ∧ σ2 = σ1;
+    mixin_val_head_step p v σ X :
+      head_step p (of_class (ExprVal v), σ) X → False;
+    mixin_call_head_step p f vs σ X :
+      head_step p (of_class (ExprCall f vs), σ) X ↔
+      (∃ (fn : func) (e2 : expr),
+        p !! f = Some fn ∧ Some e2 = apply_func fn vs ∧ X (e2, σ));
     mixin_call_in_ctx K K' e f vs :
       fill K e = fill K' (of_class (ExprCall f vs)) →
       (∃ K'', K' = comp_ectx K K'') ∨ (∃ v, of_class (ExprVal v) = e);
@@ -52,10 +53,10 @@ Section mlanguage_mixin.
       is_Some (to_class (fill K e)) → K = empty_ectx ∨ ∃ v, to_class e = Some (ExprVal v);
 
     (* [matching_expr_state] is preserved by reduction *)
-    mixin_matching_expr_state_step p e1 σ1 e2 σ2 :
+    mixin_matching_expr_state_step p e1 σ1 X :
       matching_expr_state e1 σ1 →
-      head_step p e1 σ1 e2 σ2 →
-      matching_expr_state e2 σ2;
+      head_step p (e1, σ1) X →
+      head_step p (e1, σ1) (λ '(e2, σ2), X (e2, σ2) ∧ matching_expr_state e2 σ2);
 
     (* [matching_expr_state] goes under contexts *)
     mixin_matching_expr_state_ctx K e σ :
@@ -82,10 +83,10 @@ Section mlanguage_mixin.
 
         This implies there can be only one head redex, see
         [head_redex_unique]. *)
-    mixin_step_by_val p K' K_redex e1' e1_redex σ1 e2 σ2 :
+    mixin_step_by_val p K' K_redex e1' e1_redex σ X :
       fill K' e1' = fill K_redex e1_redex →
       match to_class e1' with Some (ExprVal _) => False | _ => True end →
-      head_step p e1_redex σ1 e2 σ2 →
+      head_step p (e1_redex, σ) X →
       ∃ K'', K_redex = comp_ectx K' K'';
 
     (** If [fill K e] takes a head step, then either [e] is a value or [K] is
@@ -93,8 +94,8 @@ Section mlanguage_mixin.
         wrapping it in a context does not add new head redex positions. *)
     (* FIXME: This is the exact same conclusion as [mixin_fill_class]... is
        there some pattern or reduncancy here? *)
-    mixin_head_ctx_step_val p K e σ1 e2 σ2 :
-      head_step p (fill K e) σ1 e2 σ2 → K = empty_ectx ∨ ∃ v, to_class e = Some (ExprVal v);
+    mixin_head_ctx_step_val p K e σ X :
+      head_step p (fill K e, σ) X → K = empty_ectx ∨ ∃ v, to_class e = Some (ExprVal v);
   }.
 End mlanguage_mixin.
 
@@ -116,7 +117,7 @@ Structure mlanguage {val : Type} {public_state : Type} := Mlanguage {
   split_state : state → public_state → private_state → Prop;
   matching_expr_state : expr → state → Prop;
   apply_func : func → list val → option expr;
-  head_step : mixin_prog func → expr → state → expr → state → Prop;
+  head_step : mixin_prog func → umrel (expr * state);
 
   mlanguage_mixin :
     MlanguageMixin (val:=val) of_class to_class empty_ectx comp_ectx fill
@@ -136,7 +137,7 @@ Arguments fill {_ _ _} _ _.
 Arguments split_state {_ _ _} _ _.
 Arguments matching_expr_state {_ _ _} _ _.
 Arguments apply_func {_ _ _}.
-Arguments head_step {_ _ _} _ _ _ _ _.
+Arguments head_step {_ _ _} _.
 
 Definition expr_class {val state} (Λ : mlanguage val state) := mixin_expr_class val.
 (* A [Definition] throws off Coq's "old" ("tactic") unification engine *)
@@ -167,6 +168,7 @@ Section mlanguage.
   Implicit Types c : expr_class Λ.
   Implicit Types K : ectx Λ.
   Implicit Types p : prog Λ.
+  Implicit Types X : expr Λ * state Λ → Prop.
 
   Lemma to_of_class c : to_class (of_class Λ c) = Some c.
   Proof. apply mlanguage_mixin. Qed.
@@ -182,12 +184,12 @@ Section mlanguage.
   Lemma is_call_is_class e : is_Some (to_call e) → is_Some (to_class e).
   Proof. rewrite /to_call /is_Some. destruct (to_class e) as [[|]|]; naive_solver. Qed.
 
-  Lemma val_head_step p v σ1 e2 σ2 :
-    head_step p (of_class Λ (ExprVal v)) σ1 e2 σ2 → False.
+  Lemma val_head_step p v σ X :
+    head_step p (of_class Λ (ExprVal v), σ) X → False.
   Proof. apply mlanguage_mixin. Qed.
-  Lemma call_head_step p f vs σ1 e2 σ2 :
-    head_step p (of_class Λ (ExprCall f vs)) σ1 e2 σ2 ↔
-    ∃ fn, p !! f = Some fn ∧ Some e2 = apply_func fn vs ∧ σ2 = σ1.
+  Lemma call_head_step p f vs σ X :
+    head_step p (of_class Λ (ExprCall f vs), σ) X ↔
+    (∃ fn e2, p !! f = Some fn ∧ Some e2 = apply_func fn vs ∧ X (e2, σ)).
   Proof. apply mlanguage_mixin. Qed.
 
   Lemma fill_empty e : fill empty_ectx e = e.
@@ -199,14 +201,14 @@ Section mlanguage.
   Lemma fill_class' K e :
     is_Some (to_class (fill K e)) → K = empty_ectx ∨ ∃ v, to_class e = Some (ExprVal v).
   Proof. apply mlanguage_mixin. Qed.
-  Lemma step_by_val' p K' K_redex e1' e1_redex σ1 e2 σ2 :
+  Lemma step_by_val' p K' K_redex e1' e1_redex σ X :
       fill K' e1' = fill K_redex e1_redex →
       match to_class e1' with Some (ExprVal _) => False | _ => True end →
-      head_step p e1_redex σ1 e2 σ2 →
+      head_step p (e1_redex, σ) X →
       ∃ K'', K_redex = comp_ectx K' K''.
   Proof. apply mlanguage_mixin. Qed.
-  Lemma head_ctx_step_val' p K e σ1 e2 σ2 :
-    head_step p (fill K e) σ1 e2 σ2 → K = empty_ectx ∨ ∃ v, to_class e = Some (ExprVal v).
+  Lemma head_ctx_step_val' p K e σ X :
+    head_step p (fill K e, σ) X → K = empty_ectx ∨ ∃ v, to_class e = Some (ExprVal v).
   Proof. apply mlanguage_mixin. Qed.
   Lemma call_in_ctx K K' e f vs :
     fill K e = fill K' (of_class Λ (ExprCall f vs)) →
@@ -219,10 +221,10 @@ Section mlanguage.
     intros [H1|(x&Hx)]%call_in_ctx; auto.
     right. exists x. rewrite /to_val -Hx to_of_class//.
   Qed.
-  Lemma matching_expr_state_step p e1 σ1 e2 σ2 :
+  Lemma matching_expr_state_step p e1 σ1 X :
     matching_expr_state e1 σ1 →
-    head_step p e1 σ1 e2 σ2 →
-    matching_expr_state e2 σ2.
+    head_step p (e1, σ1) X →
+    head_step p (e1, σ1) (λ '(e2, σ2), X (e2, σ2) ∧ matching_expr_state e2 σ2).
   Proof. apply mlanguage_mixin. Qed.
   Lemma matching_expr_state_ctx K e σ :
     matching_expr_state e σ ↔ matching_expr_state (fill K e) σ.
@@ -248,37 +250,38 @@ Section mlanguage.
     intros [?|[v Hv]]%fill_class'; first by left. right.
     rewrite /to_val Hv. eauto.
   Qed.
-  Lemma step_by_val p K' K_redex e1' e1_redex σ1 e2 σ2 :
+  Lemma step_by_val p K' K_redex e1' e1_redex σ X :
       fill K' e1' = fill K_redex e1_redex →
       to_val e1' = None →
-      head_step p e1_redex σ1 e2 σ2 →
+      head_step p (e1_redex, σ) X →
       ∃ K'', K_redex = comp_ectx K' K''.
   Proof.
     rewrite /to_val => ? He1'. eapply step_by_val'; first done.
     destruct (to_class e1') as [[]|]; done.
   Qed.
-  Lemma head_ctx_step_val p K e σ1 e2 σ2 :
-    head_step p (fill K e) σ1 e2 σ2 → K = empty_ectx ∨ is_Some (to_val e).
+  Lemma head_ctx_step_val p K e σ X:
+    head_step p (fill K e, σ) X → K = empty_ectx ∨ is_Some (to_val e).
   Proof.
     intros [?|[v Hv]]%head_ctx_step_val'; first by left. right.
     rewrite /to_val Hv. eauto.
   Qed.
-  Lemma call_head_step_inv p f vs σ1 e2 σ2 :
-    head_step p (of_class Λ (ExprCall f vs)) σ1 e2 σ2 →
-    ∃ fn, p !! f = Some fn ∧ Some e2 = apply_func fn vs ∧ σ2 = σ1.
+  Lemma call_head_step_inv p f vs σ X :
+    head_step p (of_class Λ (ExprCall f vs), σ) X →
+    (∃ fn e2, p !! f = Some fn ∧ Some e2 = apply_func fn vs ∧ X (e2, σ)).
   Proof. eapply call_head_step. Qed.
-  Lemma call_head_step_intro p f vs fn σ1 er :
+  Lemma call_head_step_intro p f vs fn σ er :
     p !! f = Some fn →
     Some er = apply_func fn vs →
-    head_step p (of_call Λ f vs) σ1 er σ1.
-  Proof. intros ? ?. eapply call_head_step; eexists; eauto. Qed.
+    head_step p (of_call Λ f vs, σ) (λ '(e', σ'), e' = er ∧ σ' = σ).
+  Proof.
+    intros ? ?. eapply call_head_step; intros; simplify_eq.
+    do 2 eexists; repeat split; eauto.
+  Qed.
 
-  Definition head_reducible_no_threads (p : prog Λ) (e : expr Λ) (σ : state Λ) :=
-    ∃ e' σ', head_step p e σ e' σ'.
   Definition head_reducible (p : prog Λ) (e : expr Λ) (σ : state Λ) :=
-    ∃ e' σ', head_step p e σ e' σ'.
+    ∃ X, head_step p (e, σ) X.
   Definition head_irreducible (p : prog Λ) (e : expr Λ) (σ : state Λ) :=
-    ∀ e' σ', ¬head_step p e σ e' σ'.
+    ∀ X, ¬head_step p (e, σ) X.
   Definition head_stuck (p : prog Λ) (e : expr Λ) (σ : state Λ) :=
     to_val e = None ∧ head_irreducible p e σ.
 
@@ -287,29 +290,34 @@ Section mlanguage.
   Definition sub_redexes_are_values (e : expr Λ) :=
     ∀ K e', e = fill K e' → to_val e' = None → K = empty_ectx.
 
-  Inductive prim_step (p : prog Λ) : expr Λ → state Λ → expr Λ → state Λ → Prop :=
-    Prim_step K e1 e2 σ1 σ2 e1' e2':
-      e1 = fill K e1' → e2 = fill K e2' →
-      head_step p e1' σ1 e2' σ2 → prim_step p e1 σ1 e2 σ2.
+  Definition prim_step_mrel (p : prog Λ) : multirelation (expr Λ * state Λ) :=
+    λ '(e1, σ1) X,
+      ∃ K e1',
+        e1 = fill K e1' ∧
+        head_step p (e1', σ1) (λ '(e2', σ2), X (fill K e2', σ2)).
 
-  Lemma Prim_step' p K e1 σ1 e2 σ2 :
-    head_step p e1 σ1 e2 σ2 → prim_step p (fill K e1) σ1 (fill K e2) σ2.
-  Proof. econstructor; eauto. Qed.
+  Program Definition prim_step (p : prog Λ) : umrel (expr Λ * state Λ) :=
+    {| mrel := prim_step_mrel p |}.
+  Next Obligation.
+    intros p [e1 σ1] *.
+    intros (K & e' & -> & Hstep) HH. do 2 eexists. split_and!; eauto.
+    eapply umrel_upclosed; eauto. intros [? ?]. eauto.
+  Qed.
 
   Definition reducible (p : prog Λ) (e : expr Λ) (σ : state Λ) :=
-    ∃ e' σ', prim_step p e σ e' σ'.
+    ∃ X, prim_step p (e, σ) X.
   Definition irreducible (p : prog Λ) (e : expr Λ) (σ : state Λ) :=
-    ∀ e' σ', ¬prim_step p e σ e' σ'.
+    ∀ X, ¬ prim_step p (e, σ) X.
   Definition stuck (p : prog Λ) (e : expr Λ) (σ : state Λ) :=
     to_val e = None ∧ irreducible p e σ.
   Definition not_stuck (p : prog Λ) (e : expr Λ) (σ : state Λ) :=
     is_Some (to_val e) ∨ reducible p e σ.
+  Definition reducible_not_ub (p : prog Λ) (e : expr Λ) (σ : state Λ) :=
+    ∃ X e' σ', prim_step p (e, σ) X ∧ X (e', σ').
+  Definition not_ub (p : prog Λ) (e : expr Λ) (σ : state Λ) :=
+    is_Some (to_val e) ∨ reducible_not_ub p e σ.
 
   (** * Some lemmas about this language *)
-  Lemma prim_step_inv p e1 e2 σ1 σ2:
-    prim_step p e1 σ1 e2 σ2 →
-    ∃ K e1' e2', e1 = fill K e1' ∧ e2 = fill K e2' ∧ head_step p e1' σ1 e2' σ2.
-  Proof. inversion 1; subst; do 3 eexists; eauto. Qed.
   Lemma to_of_val v : to_val (of_val Λ v) = Some v.
   Proof. rewrite /to_val /of_val to_of_class //. Qed.
   Lemma of_to_val e v : to_val e = Some v → of_val Λ v = e.
@@ -319,7 +327,7 @@ Section mlanguage.
   Qed.
   Lemma of_to_val_flip v e : of_val Λ v = e → to_val e = Some v.
   Proof. intros <-. by rewrite to_of_val. Qed.
-  Lemma val_head_stuck p e σ e' σ': head_step p e σ e' σ' → to_val e = None.
+  Lemma val_head_stuck p e σ X: head_step p (e, σ) X → to_val e = None.
   Proof.
     destruct (to_val e) as [v|] eqn:Hval; last done.
     rewrite -(of_to_val e v) //. intros []%val_head_step.
@@ -331,9 +339,9 @@ Section mlanguage.
     - subst K. move: Hval. rewrite fill_empty. done.
     - done.
   Qed.
-  Lemma val_stuck p e σ e' σ': prim_step p e σ e' σ' → to_val e = None.
+  Lemma val_stuck p e σ X: prim_step p (e, σ) X → to_val e = None.
   Proof.
-    intros (?&?&? & -> & -> & ?%val_head_stuck)%prim_step_inv.
+    intros (K & e1' & -> & ?%val_head_stuck).
     apply eq_None_not_Some. by intros ?%fill_val%eq_None_not_Some.
   Qed.
 
@@ -350,10 +358,10 @@ Section mlanguage.
   Lemma not_reducible p e σ : ¬reducible p e σ ↔ irreducible p e σ.
   Proof. unfold reducible, irreducible. naive_solver. Qed.
   Lemma reducible_not_val p e σ : reducible p e σ → to_val e = None.
-  Proof. intros (?&?&?); eauto using val_stuck. Qed.
+  Proof. intros (?&?). eauto using val_stuck. Qed.
   Lemma val_irreducible p e σ : is_Some (to_val e) → irreducible p e σ.
-  Proof. intros [??] ? ??%val_stuck. by destruct (to_val e). Qed.
-  Global Instance of_val_inj : Inj (=) (=) (@of_val _ _ Λ).
+  Proof. intros [??] ??%val_stuck. by destruct (to_val e). Qed.
+  Global Instance of_val_inj : Inj (=) (=) (of_val Λ).
   Proof. by intros v v' Hv; apply (inj Some); rewrite -!to_of_val Hv. Qed.
   Lemma not_not_stuck p e σ : ¬not_stuck p e σ ↔ stuck p e σ.
   Proof.
@@ -364,13 +372,12 @@ Section mlanguage.
     p !! f = None →
     irreducible p (fill K (of_class Λ (ExprCall f vs))) σ.
   Proof.
-    intros ? ? Hf Hred.
-    apply prim_step_inv in Hred as (K' & e1 & e1' & Hfill & -> & Hstep).
+    intros ? X (K' & e1 & Hfill & Hstep).
     symmetry in Hfill. pose proof (call_in_ctx_to_val _ _ _ _ _ Hfill) as [[? ->]|[? ?]].
     - rewrite -fill_comp in Hfill. apply fill_inj in Hfill. subst e1.
-      pose proof (head_ctx_step_val _ _ _ _ _ _ Hstep) as [->|[? HH]].
+      pose proof (head_ctx_step_val _ _ _ _ _ Hstep) as [->|[? HH]].
       + rewrite fill_empty in Hstep.
-        apply call_head_step in Hstep as (? & ? & ? & ->). congruence.
+        apply call_head_step in Hstep as (?&?&?&?&?). congruence.
       + rewrite /to_val to_of_class // in HH.
     - apply val_head_stuck in Hstep. congruence.
   Qed.
@@ -392,35 +399,53 @@ Section mlanguage.
     head_reducible p e' σ →
     K = comp_ectx K' empty_ectx ∧ e = e'.
   Proof.
-    intros Heq (e2 & σ2 & Hred) (e2' & σ2' & Hred').
+    intros Heq (X & Hred) (X' & Hred').
     edestruct (step_by_val p K' K e' e) as [K'' HK];
       [by eauto using val_head_stuck..|].
     subst K. move: Heq. rewrite -fill_comp. intros <-%(inj (fill _)).
-    destruct (head_ctx_step_val _ _ _ _ _ _ Hred') as [HK''|[]%not_eq_None_Some].
+    destruct (head_ctx_step_val _ _ _ _ _ Hred') as [HK''|[]%not_eq_None_Some].
     - subst K''. rewrite fill_empty. done.
     - by eapply val_head_stuck.
   Qed.
 
-  Lemma head_prim_step p e1 σ1 e2 σ2 :
-    head_step p e1 σ1 e2 σ2 → prim_step p e1 σ1 e2 σ2.
-  Proof. apply Prim_step with empty_ectx; by rewrite ?fill_empty. Qed.
-
-  Lemma head_step_not_stuck p e σ e' σ':
-    head_step p e σ e' σ' → not_stuck p e σ.
-  Proof. rewrite /not_stuck /reducible /=. eauto 10 using head_prim_step. Qed.
-
-  Lemma fill_prim_step p K e1 σ1 e2 σ2 :
-    prim_step p e1 σ1 e2 σ2 → prim_step p (fill K e1) σ1 (fill K e2) σ2.
+  Lemma head_prim_step p e1 σ1 X :
+    head_step p (e1, σ1) X → prim_step p (e1, σ1) X.
   Proof.
-    intros (K' & e1' & e2' & -> & -> & ?) % prim_step_inv.
-    rewrite !fill_comp. by econstructor.
+    intros Hstep. exists empty_ectx, e1. split.
+    - by rewrite fill_empty.
+    - intros *. eapply umrel_upclosed; eauto.
+      intros [? ?]. rewrite fill_empty //.
   Qed.
+  Lemma head_step_not_stuck p e σ X:
+    head_step p (e, σ) X → not_stuck p e σ.
+  Proof. rewrite /not_stuck /reducible /=. eauto 10 using head_prim_step. Qed.
+  Lemma fill_prim_step p K e1 σ1 X X' :
+    (∀ e2 σ2, X (e2, σ2) → X' (fill K e2, σ2)) →
+    prim_step p (e1, σ1) X →
+    prim_step p (fill K e1, σ1) X'.
+  Proof.
+    intros HX (K' & e1' & -> & Hstep). rewrite fill_comp /=.
+    do 2 eexists. split_and!; eauto.
+    eapply umrel_upclosed; eauto. intros [? ?].
+    rewrite -fill_comp. eauto.
+  Qed.
+  Lemma fill_prim_step' p K e1 σ1 X :
+    prim_step p (e1, σ1) X →
+    prim_step p (fill K e1, σ1)
+        (λ '(e2', σ2), ∃ e2, e2' = fill K e2 ∧ X (e2, σ2)).
+  Proof.
+    intros Hstep. eapply fill_prim_step with (X' := λ _, _) in Hstep.
+    - eapply Hstep.
+    - intros ? ? ?. simpl. eexists. eauto.
+  Qed.
+
   Lemma fill_reducible p K e σ : reducible p e σ → reducible p (fill K e) σ.
   Proof.
-    intros (e'&σ'&?). exists (fill K e'), σ'. by apply fill_prim_step.
+    intros (X & Hstep). exists (λ '(e', σ), ∃ e, e' = fill K e ∧ X (e, σ)).
+    eapply fill_prim_step; [| apply Hstep]; eauto.
   Qed.
   Lemma head_prim_reducible p e σ : head_reducible p e σ → reducible p e σ.
-  Proof. intros (e'&σ'&?). eexists e', σ'. by apply head_prim_step. Qed.
+  Proof. intros (X&?). exists X. by apply head_prim_step. Qed.
   Lemma head_prim_fill_reducible p e K σ :
     head_reducible p e σ → reducible p (fill K e) σ.
   Proof. intro. by apply fill_reducible, head_prim_reducible. Qed.
@@ -429,16 +454,17 @@ Section mlanguage.
     rewrite -not_reducible -not_head_reducible. eauto using head_prim_reducible.
   Qed.
 
-  Lemma prim_head_step p e σ e' σ':
-    prim_step p e σ e' σ' → sub_redexes_are_values e → head_step p e σ e' σ'.
+  Lemma prim_head_step p e σ X :
+    prim_step p (e, σ) X → sub_redexes_are_values e → head_step p (e, σ) X.
   Proof.
-    intros Hprim ?. destruct (prim_step_inv _ _ _ _ _ Hprim) as (K & e1' & e2' & -> & -> & Hstep).
+    intros (K & e1' & -> & Hstep) ?.
     assert (K = empty_ectx) as -> by eauto 10 using val_head_stuck.
-    rewrite !fill_empty /head_reducible; eauto.
+    rewrite fill_empty. eapply umrel_upclosed; [apply Hstep|].
+    intros [? ?]. rewrite fill_empty //.
   Qed.
   Lemma prim_head_reducible p e σ :
     reducible p e σ → sub_redexes_are_values e → head_reducible p e σ.
-  Proof. intros (e'&σ'&Hprim) ?. do 2 eexists; by eapply prim_head_step. Qed.
+  Proof. intros (X&Hstep) ?. eexists. by eapply prim_head_step. Qed.
   Lemma prim_head_irreducible p e σ :
     head_irreducible p e σ → sub_redexes_are_values e → irreducible p e σ.
   Proof.
@@ -451,160 +477,238 @@ Section mlanguage.
     intros [] ?. split; first done. by apply prim_head_irreducible.
   Qed.
 
-  Lemma head_reducible_prim_step_ctx p K e1 σ1 e2 σ2 :
+  Lemma head_reducible_prim_step_ctx p K e1 σ1 X :
     head_reducible p e1 σ1 →
-    prim_step p (fill K e1) σ1 e2 σ2 →
-    ∃ e2', e2 = fill K e2' ∧ head_step p e1 σ1 e2' σ2.
+    prim_step p (fill K e1, σ1) X →
+    head_step p (e1, σ1) (λ '(e2', σ2), ∀ e2, e2 = fill K e2' → X (e2, σ2)).
   Proof.
-    intros (e2''&σ2''&HhstepK) (K' & e1' & e2' & HKe1 & -> & Hstep) % prim_step_inv.
+    intros (X' & HhstepK) (K' & e1' & HKe1 & Hstep).
     edestruct (step_by_val p K) as [K'' ?];
       eauto using val_head_stuck; simplify_eq/=.
     rewrite -fill_comp in HKe1; simplify_eq.
-    exists (fill K'' e2'). rewrite fill_comp; split; first done.
     apply head_ctx_step_val in HhstepK as [?|[v ?]]; simplify_eq.
-    - by rewrite !fill_empty.
+    - rewrite fill_empty. eapply umrel_upclosed; [apply Hstep|].
+      intros [e σ]. rewrite -fill_comp fill_empty //. by intros ? ? ->.
     - apply val_head_stuck in Hstep; simplify_eq.
   Qed.
 
-  Lemma head_reducible_prim_step p e1 σ1 e2 σ2 :
+  Lemma head_reducible_prim_step p e1 σ1 X :
     head_reducible p e1 σ1 →
-    prim_step p e1 σ1 e2 σ2 →
-    head_step p e1 σ1 e2 σ2.
+    prim_step p (e1, σ1) X →
+    head_step p (e1, σ1) X.
   Proof.
-    intros.
-    edestruct (head_reducible_prim_step_ctx p empty_ectx) as (?&?&?);
-      rewrite ?fill_empty; eauto.
-    by simplify_eq; rewrite fill_empty.
+    intros Hred Hpstep.
+    epose proof (head_reducible_prim_step_ctx _ empty_ectx _ _ X Hred) as Hhstep.
+    eapply umrel_upclosed.
+    - eapply Hhstep. by rewrite fill_empty.
+    - intros [e σ]. rewrite fill_empty. eauto.
   Qed.
 
   Lemma fill_stuck (P : prog Λ) e σ K : stuck P e σ → stuck P (fill K e) σ.
   Proof.
     intros Hstuck; split.
     + apply fill_not_val, Hstuck.
-    + intros e'' σ'' (K_redex &e1 &e2 &Heq &-> &Hhead)%prim_step_inv.
-      edestruct (step_by_val P K K_redex _ _ _ _ _ Heq ltac:(apply Hstuck) Hhead) as (K'' & ->).
+    + intros X (K_redex & e1 & Heq & Hhead).
+      edestruct (step_by_val P K K_redex _ _ _ _ Heq ltac:(apply Hstuck) Hhead) as (K'' & ->).
       rewrite -fill_comp in Heq. apply fill_inj in Heq as ->.
-      eapply (proj2 Hstuck). econstructor; eauto.
+      eapply (proj2 Hstuck) with (λ '(e, σ), X (fill K e, σ)).
+      do 2 eexists; split_and!; eauto.
+      eapply multirelations.umrel_upclosed; eauto. intros [? ?]. rewrite -fill_comp//.
   Qed.
 
   Lemma fill_not_stuck (P : prog Λ) e σ K : not_stuck P (fill K e) σ → not_stuck P e σ.
   Proof.
     intros [Hval | Hred].
     - left. by eapply fill_val.
-    - destruct Hred as (e' & σ' & (K_redex &e1 &e2 &Heq &-> &Hhead)%prim_step_inv).
+    - destruct Hred as (X & (K_redex & e1 & Heq & Hhead)).
       destruct (decide (to_val e = None)) as [Hnval | Hval]; first last.
       { left. destruct (to_val e) as [v | ]; by eauto. }
-      edestruct (step_by_val P K K_redex _ _ _ _ _ Heq Hnval Hhead) as (K'' & ->).
+      edestruct (step_by_val P K K_redex _ _ _ _ Heq Hnval Hhead) as (K'' & ->).
       rewrite -fill_comp in Heq. apply fill_inj in Heq as ->.
-      right. eexists _, _. econstructor; eauto.
+      right. exists (λ '(e, σ), X (fill K e, σ)). do 2 eexists; split_and!; eauto.
+      eapply multirelations.umrel_upclosed; eauto. intros [? ?]. rewrite -fill_comp//.
   Qed.
 
-  Lemma prim_step_call_inv p K f vs e' σ σ' :
-    prim_step p (fill K (of_call Λ f vs)) σ e' σ' →
-    ∃ er fn, Some er = apply_func fn vs ∧ p !! f = Some fn ∧ e' = fill K er ∧ σ' = σ.
+  Lemma prim_step_call_inv p K f vs e' σ X :
+    prim_step p (fill K (of_call Λ f vs), σ) X →
+    ∃ er fn,
+      Some er = apply_func fn vs ∧ p !! f = Some fn ∧
+      X (fill K er, σ).
   Proof.
-    intros (K' & e1 & e2 & Hctx & -> & Hstep)%prim_step_inv.
+    intros (K' & e1 & Hctx & Hstep).
     eapply step_by_val in Hstep as H'; eauto; last apply to_val_of_call.
     destruct H' as [K'' Hctx']; subst K'.
     rewrite -fill_comp in Hctx. eapply fill_inj in Hctx.
     destruct (fill_class K'' e1) as [->|Hval].
     - apply is_call_is_class. erewrite of_to_call_flip; eauto.
-    - rewrite fill_empty in Hctx. subst e1. exists e2.
-      apply call_head_step_inv in Hstep as (fn & ? & -> & ->).
-      exists fn. rewrite -fill_comp fill_empty. naive_solver.
-    - unfold is_Some in Hval. erewrite val_head_stuck in Hval; naive_solver.
+    - rewrite fill_empty in Hctx. subst e1.
+      eapply call_head_step_inv in Hstep as (?&?&?&?&HX); simplify_eq/=.
+      rewrite -fill_comp fill_empty// in HX. eauto.
+    - apply val_head_stuck in Hstep. apply not_eq_None_Some in Hval. done.
   Qed.
 
-  Lemma val_prim_step p v σ e' σ':
-   ¬ prim_step p (of_val Λ v) σ e' σ'.
+  Lemma val_prim_step p v σ X :
+   ¬ prim_step p (of_val Λ v, σ) X.
   Proof.
-    intros (K & e1' & e2' & Heq & -> & Hstep') % prim_step_inv.
+    intros (K & e1' & Heq & Hstep').
     edestruct (fill_val K e1') as (v1''& ?).
     { rewrite -Heq. rewrite to_of_val. by exists v. }
     eapply val_head_step.
     erewrite <-(of_to_val e1') in Hstep'; eauto.
   Qed.
 
-  Lemma fill_reducible_prim_step p e e' σ σ' K :
-    reducible p e σ → prim_step p (fill K e) σ e' σ' → ∃ e'', e' = fill K e'' ∧ prim_step p e σ e'' σ'.
+  Lemma fill_reducible_prim_step p e σ K X :
+    reducible p e σ →
+    prim_step p (fill K e, σ) X →
+    prim_step p (e, σ) (λ '(e2', σ2), ∀ e2, e2 = fill K e2' → X (e2, σ2)).
   Proof.
-    intros (e1 & σ1 & (K'' & e1'' & e2'' & ->  & -> & Hhead) % prim_step_inv) Hprim.
+    intros (X'' & (K'' & e1'' & -> & Hstep)) Hprim.
     rewrite fill_comp in Hprim.
-    eapply head_reducible_prim_step_ctx in Hprim as (e1' & -> & Hhead'); last by rewrite /head_reducible; eauto.
-    eexists. rewrite -fill_comp; by eauto using Prim_step'.
+    eapply head_reducible_prim_step_ctx in Hprim; last by rewrite /head_reducible; eauto.
+    do 2 eexists. split_and!; eauto.
+    eapply multirelations.umrel_upclosed; [eapply Hprim|]. intros [? ?].
+    rewrite fill_comp; eauto.
   Qed.
 
   Lemma reducible_fill p e σ K : reducible p e σ → reducible p (fill K e) σ.
+  Proof. intros (X & Hstep). eexists. eauto using fill_prim_step'. Qed.
+
+  Lemma fill_step_inv p K e1' σ1 X :
+    to_val e1' = None →
+    prim_step p (fill K e1', σ1) X →
+    prim_step p (e1', σ1) (λ '(e2', σ2), X (fill K e2', σ2)).
   Proof.
-  intros (e' & σ' & Hs).
-  inversion Hs; subst.
-  eexists (fill (comp_ectx K K0) e2'), σ'. econstructor. 1: rewrite fill_comp; reflexivity. 1: reflexivity. apply H1.
+    intros ? (K'' & e'' & Heq & Hstep).
+    eapply step_by_val in Hstep as Hstep'; eauto. destruct Hstep' as [K' ->].
+    rewrite -fill_comp in Heq. apply (inj (fill _)) in Heq as ->.
+    do 2 eexists; split_and!; eauto.
+    eapply multirelations.umrel_upclosed; eauto. intros [? ?].
+    rewrite -fill_comp//.
   Qed.
 
-  Lemma fill_step_inv K p e1' σ1 e2 σ2 :
-    to_val e1' = None → prim_step p (fill K e1') σ1 e2 σ2 →
-    ∃ e2', e2 = fill K e2' ∧ prim_step p e1' σ1 e2' σ2.
-  Proof.
-    intros H1 H2.
-    inversion H2; subst.
-    destruct (step_by_val _ _ _ _ _ _ _ _ H H1 H3) as (K'' & ->).
-    rewrite <- fill_comp in *.
-    apply fill_inj in H. subst. eexists; split; first done.
-    by econstructor.
-  Qed.
+  Lemma fill_reducible_inv p K e σ :
+    to_val e = None -> reducible p (fill K e) σ → reducible p e σ.
+  Proof. intros ? (X & Hstep%fill_step_inv); auto. eexists; eauto. Qed.
 
-  Lemma fill_inv p K e σ : to_val e = None -> reducible p (fill K e) σ -> reducible p e σ.
-  Proof.
-    intros H1 (e'&σ'&(e2'&->&H2)%fill_step_inv). 2:easy.
-    exists e2',σ'. easy.
-  Qed.
+  (* Lemma head_call_pure p f vs σ e2 σ' σ2 : *)
+  (*   head_step p (of_class Λ (ExprCall f vs), σ) σ e2 σ' → *)
+  (*   head_step p (of_class Λ (ExprCall f vs)) σ2 e2 σ2. *)
+  (* Proof. *)
+  (*   intros (fn & H1 & H2 & H3)%call_head_step. apply call_head_step. *)
+  (*   exists fn. repeat split; easy. *)
+  (* Qed. *)
 
-  Lemma head_call_pure p f vs σ e2 σ' σ2 :
-    head_step p (of_class Λ (ExprCall f vs)) σ e2 σ' -> head_step p (of_class Λ (ExprCall f vs)) σ2 e2 σ2.
-  Proof.
-    intros (fn & H1 & H2 & H3)%call_head_step. apply call_head_step.
-    exists fn. repeat split; easy.
-  Qed.
-
-  Lemma call_prim_step_fill p K f vs σ1 σ2 e2 :
-    prim_step p (fill K (of_class Λ (ExprCall f vs))) σ1 e2 σ2 →
-    ∃ (fn : func Λ) e2',
+  Lemma call_prim_step_fill p K f vs σ X :
+    prim_step p (fill K (of_class Λ (ExprCall f vs)), σ) X →
+    ∃ (fn : func Λ) e2,
       p !! f = Some fn ∧
-      apply_func fn vs = Some e2' ∧
-      e2 = fill K e2' ∧
-      σ2 = σ1.
+      apply_func fn vs = Some e2 ∧
+      X (fill K e2, σ).
   Proof.
-    intros (K' & e2' & e2'' & Hfill%eq_sym & -> & Hstep)%prim_step_inv.
+    intros (K' & e1 & Hfill%eq_sym & Hstep).
     pose proof (call_in_ctx _ _ _ _ _ Hfill) as [[K'' ->]|[? Hval]].
-    { rewrite -fill_comp in Hfill. apply fill_inj in Hfill. subst e2'.
-      pose proof (head_ctx_step_val _ _ _ _ _ _ Hstep) as [->|[? Hval]].
-      { rewrite fill_empty in Hstep. apply call_head_step in Hstep as (fn & ? & ? & ->).
+    { rewrite -fill_comp in Hfill. apply fill_inj in Hfill. subst e1.
+      pose proof (head_ctx_step_val _ _ _ _ _ Hstep) as [->|[? Hval]].
+      { rewrite fill_empty in Hstep. apply call_head_step in Hstep as (fn & ? & ? & ? & ?).
         eexists _, _; repeat split; eauto. rewrite -!fill_comp fill_empty//. }
       { exfalso. rewrite /to_val to_of_class// in Hval. } }
     { exfalso. subst. apply val_head_stuck in Hstep. rewrite /to_val to_of_class// in Hstep. }
   Qed.
 
-  Lemma call_prim_step p f vs σ1 σ2 e2 :
-    prim_step p (of_class Λ (ExprCall f vs)) σ1 e2 σ2 →
-    ∃ (fn : func Λ),
+  Lemma call_prim_step p f vs σ X :
+    prim_step p (of_class Λ (ExprCall f vs), σ) X →
+    ∃ (fn : func Λ) e2,
       p !! f = Some fn ∧
       apply_func fn vs = Some e2 ∧
-      σ2 = σ1.
+      X (e2, σ).
   Proof.
-    epose proof (call_prim_step_fill p empty_ectx _ _ _ _ _) as H.
-    rewrite fill_empty in H. intros (?&?&?&?&?&?)%H; subst.
-    eexists. repeat split; eauto. rewrite fill_empty//.
+    epose proof (call_prim_step_fill p empty_ectx _ _ _ _) as H.
+    rewrite fill_empty in H. intros (?&?&?&?&HX)%H; subst.
+    eexists _, _. repeat split; eauto. rewrite fill_empty// in HX.
   Qed.
 
-  Lemma matching_expr_state_prim_step p e1 σ1 e2 σ2 :
+  Lemma matching_expr_state_prim_step p e1 σ1 X :
     matching_expr_state e1 σ1 →
-    prim_step p e1 σ1 e2 σ2 →
-    matching_expr_state e2 σ2.
+    prim_step p (e1, σ1) X →
+    prim_step p (e1, σ1) (λ '(e2, σ2), X (e2, σ2) ∧ matching_expr_state e2 σ2).
   Proof.
-    intros Hmatch (K & e1' & e2' & -> & -> & Hstep)%prim_step_inv.
-    apply matching_expr_state_ctx in Hmatch. apply matching_expr_state_ctx.
-    eauto using matching_expr_state_step.
+    intros Hmatch (K & e1' & -> & Hstep).
+    apply matching_expr_state_ctx in Hmatch.
+    apply matching_expr_state_step in Hstep; eauto.
+    eexists K, _. repeat split; eauto. eapply multirelations.umrel_upclosed; eauto.
+    intros [? ?] [? ?]. split; eauto. by apply matching_expr_state_ctx.
   Qed.
+
+  Class IntoVal (e : expr Λ) (v : val) :=
+    into_val : of_val Λ v = e.
+
+  Class AsVal (e : expr Λ) := as_val : ∃ v, of_val Λ v = e.
+  (* There is no instance [IntoVal → AsVal] as often one can solve [AsVal] more
+  efficiently since no witness has to be computed. *)
+  Global Instance as_vals_of_val vs : TCForall AsVal (of_val Λ <$> vs).
+  Proof.
+    apply TCForall_Forall, Forall_fmap, Forall_true=> v.
+    rewrite /AsVal /=; eauto.
+  Qed.
+
+  Record pure_step p (e1 : expr Λ) (e2 : expr Λ) := {
+    pure_step_safe σ1 : reducible p e1 σ1;
+    pure_step_det σ1 X :
+      prim_step p (e1, σ1) X → X (e2, σ1)
+  }.
+
+  Class PureExec (φ : Prop) (n : nat) p (e1 : expr Λ) (e2 : expr Λ) :=
+    pure_exec : φ → relations.nsteps (pure_step p) n e1 e2.
+
+  Lemma pure_exec_fill φ n p e1 e2 K :
+    PureExec φ n p e1 e2 →
+    PureExec φ n p (fill K e1) (fill K e2).
+  Proof.
+    intros H Hφ. specialize (H Hφ). induction H as [|n x y z [Hred Hdet] Hstep IH]; econstructor.
+    - econstructor.
+      + intros σ1. destruct (Hred σ1) as (?&H). eexists. eapply fill_prim_step'; eauto.
+      + intros σ1 X HH%fill_reducible_prim_step; last apply Hred.
+        apply Hdet in HH; eauto.
+    - apply IH.
+  Qed.
+
+  Lemma pure_step_ctx p K e1 e2 :
+    pure_step p e1 e2 →
+    pure_step p (fill K e1) (fill K e2).
+  Proof.
+    intros [Hred Hstep]. split.
+    - unfold reducible in *. naive_solver eauto using fill_prim_step'.
+    - intros σ1 X HstepK. specialize (Hred σ1). specialize (Hstep σ1).
+      apply fill_reducible_prim_step in HstepK; auto.
+      apply Hstep in HstepK. eauto.
+  Qed.
+
+  Lemma pure_step_nsteps_ctx K n p e1 e2 :
+    relations.nsteps (pure_step p) n e1 e2 →
+    relations.nsteps (pure_step p) n (fill K e1) (fill K e2).
+  Proof. eauto using nsteps_congruence, pure_step_ctx. Qed.
+
+  Lemma pure_exec_ctx K P n p e1 e2 :
+    PureExec P n p e1 e2 →
+    PureExec P n p (fill K e1) (fill K e2).
+  Proof. rewrite /PureExec; eauto using pure_step_nsteps_ctx. Qed.
+
+  Record pure_head_step p (e1 : expr Λ) (e2 : expr Λ) := {
+    pure_head_step_safe σ1 : head_reducible p e1 σ1;
+    pure_head_step_det σ1 X :
+      head_step p (e1, σ1) X → X (e2, σ1)
+  }.
+
+  Lemma pure_head_step_pure_step p e1 e2 :
+    pure_head_step p e1 e2 → pure_step p e1 e2.
+  Proof.
+    intros [Hp1 Hp2]. split.
+    - intros σ. destruct (Hp1 σ) as (X & Hstep).
+      eexists. by eapply head_prim_step.
+    - intros σ X Hstep.
+      eapply head_reducible_prim_step, Hp2 in Hstep; eauto.
+  Qed.
+
 End mlanguage.
 
 (* discrete OFE instance for expr *)
